experiments/orset/out/test_opt.ml
@@ -1,0 +1,35 @@
+let _ = Random.self_init ()
+
+let random x = Z.of_int (Random.int x)
+
+let random_ops r = if (Random.int 100 < r) then (random 1000000, Orset_opt.Add (random 100))
+  else (random 1000000, Orset_opt.Rem (random 100))
+
+let pick_r r r1 r2 = if (Random.int 100 < r) then r1 else r2
+
+let app_op set op = (Orset_opt.app_op set op)
+
+let merge lca a b = Orset_opt.merge1 lca a b
+
+let rec test lca a b count =
+  if count = 0 then () else
+  let lca = merge lca a b in
+  let replica_ratio = 50 in
+  let insert_ratio = 50 in
+  let merge_ratio = 500 in
+  let (a, b) = if pick_r replica_ratio a b = a then (app_op a (random_ops insert_ratio), b) else (a, app_op b (random_ops insert_ratio)) in
+  let lca = if (count mod merge_ratio = 0) then merge lca a b else lca in
+  test lca a b (count-1)
+
+let rec gen_list acc x =
+  if x = 0 then acc else
+    gen_list ((random 100000, random 1000)::acc) (x-1)
+
+let _ =
+  Memtrace.trace_if_requested ();
+  let lca = gen_list [] 1000 in
+  let a = lca in
+  let b = lca in
+  test lca a b 10000
+
+
